Update to variant, and add record

shift-reset/core/syntax.v
@@ -47,7 +47,7 @@ Inductive term : Type :=
 | TPerform : val_term -> term
 | THandle : term -> ret_term -> eff_term -> term
 | TShallowHandle : term -> ret_term -> eff_term -> term
-| TPolyMatch : val_term -> poly_variant_term -> term
+| TMatch : val_term -> variant_term -> term
 with term1 : Type :=
 | T1 : binder -> term -> term1
 with term2 : Type :=
@@ -75,7 +75,9 @@ with val_term : Type :=
 | TVAssert : val_term -> val_term
 | TVOp1 : op1 -> val_term -> val_term
 | TVOp2 : op2 -> val_term -> val_term -> val_term
-| TVPolyVariant : tag -> list val_term -> val_term
+| TVVariant : tag -> list val_term -> val_term
+| TVRecord : record_term -> val_term
+| TVProj : val_term -> tag -> val_term
 with ret_term : Type :=
 | TRetNone : ret_term
 | TRetSome : binder -> term -> ret_term
@@ -85,9 +87,12 @@ with exn_term : Type :=
 with eff_term : Type :=
 | TEffLast : pattern -> binder -> term -> eff_term
 | TEffCons : pattern -> binder -> term -> eff_term -> eff_term
-with poly_variant_term : Type :=
-| TPolyVariantNil : poly_variant_term
-| TPolyVariantCons : pattern -> term -> poly_variant_term -> poly_variant_term.
+with variant_term : Type :=
+| TVariantNil : variant_term
+| TVariantCons : pattern -> term -> variant_term -> variant_term
+with record_term : Type :=
+| TRecordNil : record_term
+| TRecordCons : tag -> val_term -> record_term -> record_term.
 
 Inductive val : Type :=
 | VUnit : val
@@ -106,7 +111,8 @@ Inductive val : Type :=
 | VMKPure : metakont -> val
 | VMKReset : metakont -> tag -> val
 | VMKHandle : metakont -> handle_clo -> val
-| VPolyVariant : poly_variant -> val
+| VVariant : variant -> val
+| VRecord : record -> val
 with fun_clo : Type :=
 | CFun : env -> term1 -> fun_clo
 with fix_clo : Type :=
@@ -138,5 +144,8 @@ with exn : Type :=
 | Exn : tag -> list val -> exn
 with eff : Type :=
 | Eff : tag -> list val -> eff
-with poly_variant : Type :=
-| PolyVariant : tag -> list val -> poly_variant.
+with variant : Type :=
+| Variant : tag -> list val -> variant
+with record : Type :=
+| RecordNil : record
+| RecordCons : tag -> val -> record -> record.
