shift-reset/core/record.v
@@ -1,0 +1,7 @@
+From shift_reset.core Require Import syntax tag.
+
+Fixpoint record_lookup (tag : tag) (r : record) : option val :=
+  match r with
+  | RecordNil => None
+  | RecordCons tag' v r' => if tag_eqb tag tag' then Some v else record_lookup tag r'
+  end.
