shift-reset/core/val.v
@@ -13,8 +13,8 @@ Definition VExn' (tag : tag) (vs : list val) : val :=
 Definition VEff' (tag : tag) (vs : list val) : val :=
   VEff (Eff tag vs).
 
-Definition VPolyVariant' (tag : tag) (vs : list val) : val :=
-  VPolyVariant (PolyVariant tag vs).
+Definition VVariant' (tag : tag) (vs : list val) : val :=
+  VVariant (Variant tag vs).
 
 Definition VBool (b : bool) : val :=
   if b then VTrue else VFalse.
