shift-reset/interpreter/dispatch.v
@@ -168,7 +168,8 @@ Fixpoint equal_val (v1 v2 : val) : imonad bool :=
   | VRef l1, VRef l2 => imonad_pure (loc_eqb l1 l2)
   | VExn exn1, VExn exn2 => equal_exn exn1 exn2
   | VEff eff1, VEff eff2 => equal_eff eff1 eff2
-  | VPolyVariant pv1, VPolyVariant pv2 => equal_poly_variant pv1 pv2
+  | VVariant v1', VVariant v2' => equal_variant v1' v2'
+  | VRecord r1, VRecord r2 => equal_record r1 r2
   | _, _ => imonad_throw_error (Type_error "equal_val")
   end
 with equal_exn (exn1 exn2 : exn) : imonad bool :=
@@ -179,10 +180,20 @@ with equal_eff (eff1 eff2 : eff) : imonad bool :=
   let (tag1, vs1) := eff1 in
   let (tag2, vs2) := eff2 in
   if tag_eqb tag1 tag2 then equal_val_list_aux equal_val vs1 vs2 else imonad_pure false
-with equal_poly_variant (pv1 pv2 : poly_variant) : imonad bool :=
-  let (tag1, vs1) := pv1 in
-  let (tag2, vs2) := pv2 in
-  if tag_eqb tag1 tag2 then equal_val_list_aux equal_val vs1 vs2 else imonad_pure false.
+with equal_variant (v1 v2 : variant) : imonad bool :=
+  let (tag1, vs1) := v1 in
+  let (tag2, vs2) := v2 in
+  if tag_eqb tag1 tag2 then equal_val_list_aux equal_val vs1 vs2 else imonad_pure false
+with equal_record (r1 r2 : record) : imonad bool :=
+  match r1, r2 with
+  | RecordNil, RecordNil => imonad_pure true
+  | RecordCons tag1 v1 r1', RecordCons tag2 v2 r2' =>
+      if tag_eqb tag1 tag2 then
+        b <- equal_val v1 v2;
+        if b then equal_record r1' r2' else imonad_pure false
+      else imonad_pure false
+  | _, _ => imonad_pure false
+  end.
 
 Definition vprod_equal (v1 v2 arg : val) : imonad bool :=
   p <- unwrap_vprod arg;
@@ -210,8 +221,11 @@ Definition vexn_equal (exn : exn) (arg : val) : imonad bool :=
 Definition veff_equal (eff : eff) (arg : val) : imonad bool :=
   unwrap_veff arg >>= equal_eff eff.
 
-Definition vpoly_variant_equal (pv : poly_variant) (arg : val) : imonad bool :=
-  unwrap_vpoly_variant arg >>= equal_poly_variant pv.
+Definition vvariant_equal (v : variant) (arg : val) : imonad bool :=
+  unwrap_vvariant arg >>= equal_variant v.
+
+Definition vrecord_equal (r : record) (arg : val) : imonad bool :=
+  unwrap_vrecord arg >>= equal_record r.
 
 Definition vunit_ltb (arg : val) : imonad val :=
   VFalse <$ unwrap_vunit arg.
@@ -375,11 +389,17 @@ Definition veff_eqb (eff : eff) (arg : val) : imonad val :=
 Definition veff_neqb (eff : eff) (arg : val) : imonad val :=
   VBool_by negb <$> veff_equal eff arg.
 
-Definition vpoly_variant_eqb (pv : poly_variant) (arg : val) : imonad val :=
-  VBool <$> vpoly_variant_equal pv arg.
+Definition vvariant_eqb (v : variant) (arg : val) : imonad val :=
+  VBool <$> vvariant_equal v arg.
 
-Definition vpoly_variant_neqb (pv : poly_variant) (arg : val) : imonad val :=
-  VBool_by negb <$> vpoly_variant_equal pv arg.
+Definition vvariant_neqb (v : variant) (arg : val) : imonad val :=
+  VBool_by negb <$> vvariant_equal v arg.
+
+Definition vrecord_eqb (r : record) (arg : val) : imonad val :=
+  VBool <$> vrecord_equal r arg.
+
+Definition vrecord_neqb (r : record) (arg : val) : imonad val :=
+  VBool_by negb <$> vrecord_equal r arg.
 
 Definition dispatch_ltb (v : val) : imonad (val -> imonad val) :=
   match v with
@@ -446,7 +466,8 @@ Definition dispatch_eqb (v : val) : imonad (val -> imonad val) :=
   | VRef l => imonad_pure (vref_eqb l)
   | VExn exn => imonad_pure (vexn_eqb exn)
   | VEff eff => imonad_pure (veff_eqb eff)
-  | VPolyVariant pv => imonad_pure (vpoly_variant_eqb pv)
+  | VVariant v' => imonad_pure (vvariant_eqb v')
+  | VRecord r => imonad_pure (vrecord_eqb r)
   | _ => imonad_throw_error (Type_error "dispatch_eqb")
   end.
 
@@ -463,7 +484,8 @@ Definition dispatch_neqb (v : val) : imonad (val -> imonad val) :=
   | VRef l => imonad_pure (vref_neqb l)
   | VExn exn => imonad_pure (vexn_neqb exn)
   | VEff eff => imonad_pure (veff_neqb eff)
-  | VPolyVariant pv => imonad_pure (vpoly_variant_neqb pv)
+  | VVariant v' => imonad_pure (vvariant_neqb v')
+  | VRecord r => imonad_pure (vrecord_neqb r)
   | _ => imonad_throw_error (Type_error "dispatch_neqb")
   end.
 
